@prefix rdfs: <http://www.w3.org/2000/01/rdf-schema#> .
@prefix rdf: <http://www.w3.org/1999/02/22-rdf-syntax-ns#> .
@prefix auto: <http://program/automaton#> .
@prefix owl: <http://www.w3.org/2002/07/owl#> .
@prefix xsd: <http://www.w3.org/2001/XMLSchema#> .

auto:command
	a owl:Class ;
        #rdfs:subClassOf owl:NamedIndividual ;
	#rdfs:subClassOf <https://schema.org/SoftwareApplication> ;
	rdfs:comment "The resource is executable by a machine." .

auto:executable
	a owl:Class ;
	rdfs:subClassOf auto:command ;
	rdfs:comment "arguments are set. Use another auto:command for custom arguments. link to this resource via auto:execute" ;
	rdfs:comment "per commandline executable." .


auto:loadable
	rdfs:comment "Deprecated, dont use";
	a owl:Property ;
	rdfs:comment """
		Is true, when eg file exists and is available or if the 
		internetresource can be accessed.
		"""" ;
	rdfs:comment "Is false, eg if file could be created but isnt created yet" .

auto:argument
	rdfs:comment """argument of a auto:command. 
		Explains the use and sets the used input""" ;
	rdfs:comment """
		to alterate argument create new auto:command 
		with new auto:argument and link this new argument per 
		auto:overwrite to original
		""" ;
	rdfs:seeAlso auto:command, auto:uses, auto:overwrite;
	rdfs:subClassOf [ a owl:Restriction ;
			owl:onDataDomain auto:uses ;
			owl:minCardinality 1 ] ;
	rdfs:subClassOf [ a owl:Restriction ; 
			owl:onDataRange auto:default ; 
			owl:maxCardinality 1 ] ;
	rdfs:subClassOf [ a owl:Restriction ;
			owl:onDataDomain auto:overwrite ;
			owl:maxCardinality 1 ] ;
	rdfs:subClassOf [ a owl:Restriction ;
			owl:onDataDomain auto:keyword ;
			owl:maxCardinality 1 ] ;
	rdfs:subClassOf [ a owl:Restriction ;
			owl:onDataDomain auto:index ;
			owl:maxCardinality 1 ] ;
	rdfs:comment "class for arguments for executable" .

auto:uses a owl:ObjectProperty ;
	rdfs:comment "source-command uses an argument described by target" ;
	rdfs:domain auto:command ;
	rdfs:range auto:argument .

auto:overwrite
	a owl:ObjectProperty;
	rdfs:comment "Points which variable of a program will be overwritten by an argument of established command" ;
	rdfs:seeAlso auto:execute ;
	rdfs:domain auto:argument ;
	rdfs:range auto:argument .

auto:keyword
	rdfs:comment "string to identify given parameter" ;
	rdfs:domain auto:argument ;
	rdfs:range rdfs:Literal .

auto:index
	rdfs:comment "position of argument, when calling command" ;
	rdfs:range xsd:nonNegativeInteger .

auto:default
	rdf:type rdf:Property ;
	rdfs:comment "Resource used for input." ;
	rdfs:seeAlso auto:default_value, auto:default_target .

auto:default_value
	rdf:type owl:ObjectProperty ;
	rdfs:comment "Uses Literal directly as argument" ;
	rdfs:subPropertyOf auto:default .

auto:default_target
	rdf:type owl:DatatypeProperty ;
	rdfs:comment "Uses content of resource for argument. " ;
	rdfs:comment "eg. files will be provided for writing and reading." ;
	rdfs:subPropertyOf auto:default ;
	owl:propertyDisjointWith auto:default_value .

auto:execute
	a owl:ObjectProperty ;
	rdfs:comment "command builts upon other command but overwrite arguments";
	rdfs:seeAlso auto:overwrite ;
	rdfs:domain auto:command ;
	rdfs:range auto:executable .


## These Resources are used to describe newly generated Resources by commands

auto:generates
	a rdf:Property ;
	a owl:ObjectProperty ;
	rdfs:comment "points the variable container towards a placeholder for the generated data" ;
	rdfs:comment "Is used for generating information about new/old resources" ;
	rdfs:Domain auto:argument ;
	rdfs:Range auto:generatabledata .



auto:generatabledata
	a rdf:Class ;
	rdfs:comment "Is used for generating information about new resources" ;
	rdfs:comment "labels a placeholder for data, that is generated by auto:program" .


auto:originates
	rdfs:comment "used for ontology to create a logical link for property-transmission" ;
        owl:propertyChainAxiom ( [ owl:inverseOf auto:created ] auto:overwrite auto:generates ) ;
        #owl:propertyChainAxiom ( [ owl:inverseOf auto:default_target ] auto:overwrite auto:generates ) ;
	rdf:type owl:ObjectProperty .
	

auto:inputinformation
	rdfs:comment "I think this is unuseful" ;
	a rdf:Property ;
	rdfs:comment "Is used for generating information about new resources" ;
	rdfs:comment "Is used for automatic finding viable input for variable" ;
	rdfs:comment "Points to a placeholder for data, that is used as input by auto:program" .

auto:created
	a rdf:Property;
	rdfs:comment "If program creates file, this links from corresponding argument to the file-resource" ;
	rdfs:comment "is created by useprogram.interpolate_newinformation" ;
	rdfs:comment "is used by logic, when ascertaining, newinformation about resources" ;
	rdfs:range auto:argument ;
	rdfs:domain auto:generatabledata ;
	a owl:ObjectProperty . #else owlready2 makes problems


## Here i will implement all complex program implementation

auto:complex_program_linearfactory rdfs:subClassOf auto:command ;
	rdfs:comment "complex program, consisting of several subprograms" ;
	rdfs:comment "can be automaticly created by just naming wanted output and commands, that are usable" ;
	rdfs:SeeAlso <python://rdfprogram.pathfinder.main> .

auto:factorypart a rdf:Property ;
	rdfs:comment "commands that are used" ;
	rdfs:domain auto:complex_program_linearfactory ;
	rdfs:range auto:command .

#Wont implement auto:input has no immediate usecases
#auto:input rdfs:subClassOf auto:uses ;
#	rdfs:comment "Marks the inputresources for a auto:command" .

auto:output rdfs:subClassOf auto:uses ;
	rdfs:comment "Marks the outputresources of a auto:command" ;
	rdfs:domain auto:command .

#this is needed for automatic generation for graph

auto:generation_target
	a owl:Class ;
	rdfs:comment "things that have to be generated".

auto:generation_successful
	a owl:class ;
	rdfs:comment "things that have been generated".

